add MPLS proofs

deps/poulet4/lib/P4automata/Benchmarks/MPLSVectorizedProof.v
@@ -1,20 +1,222 @@
-Require Import Poulet4.P4automata.Examples.ProofHeader.
-Require Import Poulet4.P4automata.Examples.MPLSVectorized.
+Require Import Poulet4.P4automata.Benchmarks.ProofHeader.
+Require Import Poulet4.P4automata.Benchmarks.MPLSVectorized.
 
-Lemma prebisim_mpls_unroll:
-  pre_bisimulation MPLSVect.aut
-                   (WPSymLeap.wp (H:=_))
-                   (separated _ _ _ MPLSVect.aut)
-                   nil
-                   (mk_init 10 MPLSVect.aut MPLSPlain.ParseMPLS MPLSUnroll.ParseMPLS0)
-                   (inl (inl MPLSPlain.ParseMPLS), [], [])
-                   (inl (inr MPLSUnroll.ParseMPLS0), [], []).
-Proof.
-  set (rel0 := mk_init 10 MPLSVect.aut MPLSPlain.ParseMPLS MPLSUnroll.ParseMPLS0).
-  cbv in rel0.
-  subst rel0.
-  time (repeat solve_bisim).
-  cbv in *.
-  intuition (try congruence).
-Time Qed. 
 
+
+Module PlainUnroll.
+
+  Notation A := MPLSVect.aut.
+  Notation conf := (P4automaton.configuration (P4A.interp A)).
+
+  Definition r_states :=
+    Eval vm_compute in (Reachability.reachable_states
+                          A
+                          200
+                          MPLSPlain.ParseMPLS
+                          MPLSUnroll.ParseMPLS0).
+
+  Definition top : Relations.rel conf := fun _ _ => True.
+  Definition top' : Relations.rel (state_template A) := fun _ _ => True.
+
+  Declare ML Module "mirrorsolve".
+
+  RegisterPrim (@TVar (sig A) (CEmp _) (Bits 0)) "p4a.core.var".
+  RegisterPrim (@TFun (sig A) (CEmp _) [] (Bits 0)) "p4a.core.fun".
+
+  RegisterPrim (@VHere (sig A) (CEmp _) (Bits 0)) "p4a.core.vhere".
+  RegisterPrim (@VThere (sig A) (CEmp _) (Bits 0) (Bits 0)) "p4a.core.vthere".
+
+
+  RegisterPrim (@FEq (sig A) (CEmp _) (Bits 0)) "p4a.core.eq".
+  RegisterPrim (@FTrue (sig A) (CEmp _)) "p4a.core.tt".
+  RegisterPrim (@FFalse (sig A) (CEmp _)) "p4a.core.ff".
+  RegisterPrim (@FRel (sig A) (CEmp _)) "p4a.core.rel".
+  RegisterPrim (@FNeg (sig A) (CEmp _)) "p4a.core.neg".
+  RegisterPrim (@FOr (sig A) (CEmp _)) "p4a.core.or".
+  RegisterPrim (@FAnd (sig A) (CEmp _)) "p4a.core.and".
+  RegisterPrim (@FForall (sig A) (CEmp _)) "p4a.core.forall".
+
+  RegisterPrim (@FImpl (sig A) (CEmp _)) "p4a.core.impl".
+
+  RegisterPrim (@CEmp (sig A)) "p4a.core.cnil".
+  RegisterPrim (@CSnoc (sig A)) "p4a.core.csnoc".
+
+  RegisterPrim (@inl nat bool) "coq.core.inl".
+  RegisterPrim (@inr nat bool) "coq.core.inr".
+
+  RegisterPrim FirstOrderConfRelSimplified.Bits "p4a.sorts.bits".
+  RegisterPrim FirstOrderConfRelSimplified.Store "p4a.sorts.store".
+
+  RegisterPrim FirstOrderConfRelSimplified.BitsLit "p4a.funs.bitslit".
+  RegisterPrim FirstOrderConfRelSimplified.Concat "p4a.funs.concat".
+  RegisterPrim FirstOrderConfRelSimplified.Slice "p4a.funs.slice".
+  RegisterPrim FirstOrderConfRelSimplified.Lookup "p4a.funs.lookup".
+
+  RegisterPrim (@HList.HNil nat (fun _ => bool)) "p4a.core.hnil".
+  RegisterPrim (@HList.HCons nat (fun _ => bool)) "p4a.core.hcons".
+
+  ClearEnvCtors.
+
+  RegisterEnvCtors 
+    (MPLSPlain.HdrMPLS0, FirstOrderConfRelSimplified.Bits 32) 
+    (MPLSPlain.HdrMPLS1, FirstOrderConfRelSimplified.Bits 32)  
+    (MPLSPlain.HdrUDP, FirstOrderConfRelSimplified.Bits 32)   
+    (MPLSUnroll.HdrMPLS0, FirstOrderConfRelSimplified.Bits 32) 
+    (MPLSUnroll.HdrMPLS1, FirstOrderConfRelSimplified.Bits 32)  
+    (MPLSUnroll.HdrUDP, FirstOrderConfRelSimplified.Bits 32).
+
+  Lemma prebisim_mpls_unroll:
+    pre_bisimulation A
+                    (wp r_states)
+                    top
+                    []
+                    [BCEmp, ⟨ inr false, 0 ⟩ ⟨ inr true, 0 ⟩ ⊢ bfalse;
+                      BCEmp, ⟨ inr true, 0 ⟩ ⟨ inr false, 0 ⟩ ⊢ bfalse]
+                    {| cr_st := {|
+                          cs_st1 := {|
+                            st_state := inl (inl (MPLSPlain.ParseMPLS));
+                            st_buf_len := 0;
+                          |};
+                          cs_st2 := {|
+                            st_state := inl (inr (MPLSUnroll.ParseMPLS0));
+                            st_buf_len := 0;
+                          |};
+                        |};
+                        cr_ctx := BCEmp;
+                        cr_rel := btrue;
+                    |}.
+  Proof.
+    time "build phase" repeat (time "single step" run_bisim top top' r_states).
+    time "close phase" close_bisim top'.
+  Time Admitted. 
+End PlainUnroll.
+
+Module VectUnroll.
+
+  Notation A := MPLSVectUnroll.aut.
+  Notation conf := (P4automaton.configuration (P4A.interp A)).
+
+  Definition r_states :=
+    Eval vm_compute in (Reachability.reachable_states
+                          A
+                          200
+                          MPLSPlain.ParseMPLS
+                          MPLSInline.ParseMPLS).
+
+  Definition top : Relations.rel conf := fun _ _ => True.
+  Definition top' : Relations.rel (state_template A) := fun _ _ => True.
+
+  ClearEnvCtors.
+
+  RegisterEnvCtors 
+    (MPLSPlain.HdrMPLS0, FirstOrderConfRelSimplified.Bits 32) 
+    (MPLSPlain.HdrMPLS1, FirstOrderConfRelSimplified.Bits 32)  
+    (MPLSPlain.HdrUDP, FirstOrderConfRelSimplified.Bits 32)   
+    (MPLSInline.HdrMPLS0, FirstOrderConfRelSimplified.Bits 32) 
+    (MPLSInline.HdrMPLS1, FirstOrderConfRelSimplified.Bits 32)  
+    (MPLSInline.HdrUDP, FirstOrderConfRelSimplified.Bits 32).
+
+  Lemma prebisim_mpls_inline:
+    pre_bisimulation A
+                    (wp r_states)
+                    top
+                    []
+                    [BCEmp, ⟨ inr false, 0 ⟩ ⟨ inr true, 0 ⟩ ⊢ bfalse;
+                      BCEmp, ⟨ inr true, 0 ⟩ ⟨ inr false, 0 ⟩ ⊢ bfalse]
+                    {| cr_st := {|
+                          cs_st1 := {|
+                            st_state := inl (inl (MPLSPlain.ParseMPLS));
+                            st_buf_len := 0;
+                          |};
+                          cs_st2 := {|
+                            st_state := inl (inr (MPLSInline.ParseMPLS));
+                            st_buf_len := 0;
+                          |};
+                        |};
+                        cr_ctx := BCEmp;
+                        cr_rel := btrue;
+                    |}.
+  Proof.
+    time "build phase" repeat (time "single step" run_bisim top top' r_states).
+    time "close phase" close_bisim top'.
+  Time Admitted. 
+End VectUnroll.
+
+Module UnrollInline.
+
+  Notation A := MPLSUnrollInline.aut.
+  Notation conf := (P4automaton.configuration (P4A.interp A)).
+
+  Definition r_states :=
+    Eval vm_compute in (Reachability.reachable_states
+                          A
+                          200
+                          MPLSUnroll.ParseMPLS0
+                          MPLSInline.ParseMPLS).
+
+  Definition top : Relations.rel conf := fun _ _ => True.
+  Definition top' : Relations.rel (state_template A) := fun _ _ => True.
+
+  ClearEnvCtors.
+
+  RegisterEnvCtors 
+    (MPLSUnroll.HdrMPLS0, FirstOrderConfRelSimplified.Bits 32) 
+    (MPLSUnroll.HdrMPLS1, FirstOrderConfRelSimplified.Bits 32)  
+    (MPLSUnroll.HdrUDP, FirstOrderConfRelSimplified.Bits 32)   
+    (MPLSInline.HdrMPLS0, FirstOrderConfRelSimplified.Bits 32) 
+    (MPLSInline.HdrMPLS1, FirstOrderConfRelSimplified.Bits 32)  
+    (MPLSInline.HdrUDP, FirstOrderConfRelSimplified.Bits 32).
+
+  Lemma prebisim_mpls_inline:
+    pre_bisimulation A
+                    (wp r_states)
+                    top
+                    []
+                    [BCEmp, ⟨ inr false, 0 ⟩ ⟨ inr true, 0 ⟩ ⊢ bfalse;
+                      BCEmp, ⟨ inr true, 0 ⟩ ⟨ inr false, 0 ⟩ ⊢ bfalse]
+                    {| cr_st := {|
+                          cs_st1 := {|
+                            st_state := inl (inl (MPLSUnroll.ParseMPLS0));
+                            st_buf_len := 0;
+                          |};
+                          cs_st2 := {|
+                            st_state := inl (inr (MPLSInline.ParseMPLS));
+                            st_buf_len := 0;
+                          |};
+                        |};
+                        cr_ctx := BCEmp;
+                        cr_rel := btrue;
+                    |}.
+  Proof.
+    time "build phase" repeat (time "single step" run_bisim top top' r_states).
+    time "close phase" close_bisim top'.
+  Time Admitted. 
+
+  (* Definition r_states' :=
+    Eval vm_compute in (Reachability.reachable_states
+                          A
+                          200
+                          MPLSUnroll.ParseMPLS1
+                          MPLSInline.ParseMPLS).
+  Goal pre_bisimulation A
+      (wp r_states)
+      top
+      []
+      [BCEmp, ⟨ inr false, 0 ⟩ ⟨ inr true, 0 ⟩ ⊢ bfalse;
+        BCEmp, ⟨ inr true, 0 ⟩ ⟨ inr false, 0 ⟩ ⊢ bfalse]
+      {| cr_st := {|
+            cs_st1 := {|
+              st_state := inl (inl (MPLSUnroll.ParseMPLS1));
+              st_buf_len := 0;
+            |};
+            cs_st2 := {|
+              st_state := inl (inr (MPLSInline.ParseMPLS));
+              st_buf_len := 0;
+            |};
+          |};
+          cr_ctx := BCEmp;
+          cr_rel := btrue;
+      |}.
+  Proof.
+    time "build phase" repeat (time "single step" run_bisim top top' r_states'). *)
+End UnrollInline.
