deps/poulet4/lib/P4automata/Benchmarks/SmallFilterProof.v
@@ -79,4 +79,4 @@ Lemma prebisim_incremental_sep:
 Proof.
   time "build phase" repeat (time "single step" run_bisim top top' r_states).
   time "close phase" close_bisim top'.
-Admitted.
+Time Admitted.
